Suppose c is a constant, $\lim_{ x \to a } f(x)$ and $\lim_{ x \to a } g(x)$ is defined

1. $\lim_{ x \to a }[f(x) \pm g(x)] = \lim_{ x \to a } \pm \lim_{ x \to a } g(x)$
2. $\lim_{ x \to a } c \ f(x) = c \ \lim_{ x \to a } f(x)$
3. $\lim_{ x \to a }[f(x)g(x)] = \lim_{ x \to a } f(x) \ \lim_{ x \to a } g(x)$
4. $\lim_{ x \to a }\left[ \frac{f(x)}{g(x)} \right] = \frac{{\lim_{ a \to a } f(x)}}{\lim_{ x \to a }g(x)}$
5. $\lim_{ x \to a }[f(x)]^n = [\lim_{ x \to a }f(x)]^n$
6. $\lim_{ x \to a }c = c$
7. $\lim_{ x \to a }x=a$
8. $\lim_{ x \to a }x^n = a^n$

##### Example 1:
$$
\lim_{ x \to 1 } f(x) = 3, \ \lim_{ x \to -1 } g(x) = -2  
$$
Find:
$$
\lim_{ x \to -1 }[3f(x)- 2g(x)] = 3\lim_{ x \to 1 }f(x) - 2\lim_{ x \to -1 }g(x)
$$
$$
= 6 - 2(-2) = 13
$$
##### Example 2:
$$
\lim_{ x \to 5 }(2x^2-3x+4) = 2(5)^2-3(5)+4=39
$$
##### Example 3:
$$
\lim_{ x \to -2 } \frac{{x^3+2x-1}}{5-3(-2)}
$$
##### Definition: A function of the form $\frac{polynomail}{polynomail}$ is called a rational function

## Direction Substitution Property
---
If a $f(x)$ is a polynomial or a rational function, and a is in its domain then $\lim_{ x \to a }f(x) = f(a)$. If this happens, f is continuous at a

## Finding Limits of (non-piecewise) Functions
---
$\lim_{ x \to a }f(x)$: Direct substitution
	(a). f(a) is defined: $\lim_{ x \to a } f(x) = f(a)$
	(b). f(a) = $\frac{0}{0}$ -> Algebra! 
		(i). Factoring
			Ex. $\lim_{ x \to 1 } \frac{{x^2 -1}}{x-1}$ with D.S. this equals $\frac{0}{0}$
			$= \lim_{ x \to 1 } \frac{{(x-1)(x+1)}}{x-1} = \lim_{ x \to 1} (x+1)$
			$= 2$
		(ii). Rationalizing
			Ex. $\lim_{ t \to 0 } \frac{{\sqrt{ t^2 + 9 } -3 }}{t^2}$ with D.S equals $\frac{0}{0}$
			Need to multiply by the conjugate (flipping the signs)
			$= \lim_{ t \to 0 } \frac{{t^2 + 9 - 9}}{t^2(\sqrt{ t^2 +9 } +3)}$
			$= \lim_{ t \to 0 } \frac{{t^2}}{t^2(\sqrt{ t^2 + 9} +3)}$
			$= \lim_{ t \to 0 } \frac{{1}}{\sqrt{ t^2 +9 } +3}$
			$= \frac{1}{6}$
		(iii). Simplify fractions
			Ex. $\lim_{ x \to 0 } \frac{\frac{1}{3+x} - \frac{1}{3}}{x}$
			= $\lim_{ x \to 0 } \frac{\frac{1*3}{(x+3)*3}-\frac{3+x}{(x+3)*3}}{x}$
			= $\lim_{ x \to 0 }\frac{{\frac{{3-3-x}}{3(x+3)}}}{x}$
			= ${\lim_{ x \to 0 }\lim_{ x \to 0 }\frac{-x}{3(x+3)}}(\frac{1}{x})$
			= $\lim_{ x \to 0 }-\frac{-1}{3(x+3)}$
			= $substitution -\frac{1}{3(3)}=-\frac{1}{9}$
	(c). D.S -> $\frac{c}{0}, c\ne 0$
		  Infinite limit
		  Determine $\lim_{ x \to a^+ }$ and $\lim_{ x \to a^- }$
		  Both $\pm \infty \to \pm \infty$
		  One is $+\infty$, other is $-\infty$
		  then DNE

##### Example 1.
$$
\lim_{ x \to -2 } \frac{-4}{x+2}
$$
With direct substitution it equals 0:
$$
\lim_{ x \to -2 } \frac{{-4}}{0} 
$$
So now we have to approach it from both sides:
Left side:
$$
\lim_{ x \to -2^- } \frac{{-4}}{x+2} = \infty
$$
Right side
$$
\lim_{ x \to -2^+ } \frac{{-4}}{x+2} = - \infty
$$
These are two different answers so $\lim_{ x \to -2 } = DNE$

##### Example 2.
$$
\lim_{ x \to 0 } \frac{6}{x^2} 
$$
With direct substitution it equals 0:
$$
\lim_{ x \to 0 } \frac{6}{0} 
$$
So we have to approach it from both sides:
Left side:
$$
\lim_{ x \to 0^- } \frac{6}{x^2} = + \infty  
$$
Right side:
$$
\lim_{ x \to 0^+ } \frac{6}{x^2} = + \infty 
$$
They're the same so $\lim_{ x \to 0 } = + \infty$

##### Example 3.
$$
\lim_{ x \to -1 } \frac{{-z-3}}{(z+1)^2} 
$$
With direct substitution it equals 0:
$$
\lim_{ x \to -1 } -\frac{2}{0} 
$$
So we have to approach it from both sides:
Left side:
$$
\lim_{ x \to -1^- } \frac{{-z-3}}{(z+1)^2} = - \infty
$$
$-z-3$ is negative because if you plug in something a little to the left of -1 you get a negative
$(z+3)^2$ is positive because its squared
so f(x) is negative because a positive and a negative is a negative
$$
\lim_{ x \to -1^+ } \frac{{-z-3}}{(x+1)^2} = - \infty
$$
$-z-3$ is negative because if you plug in something a little to the right of -1 you get a negative
$(z+3)^2$ is positive because its squared
so f(x) is negative because a positive and a negative is a negative

They're the same so $\lim_{ x \to -1 } = -\infty$

##### Example 4:
$$
\lim_{ x \to 3 } \frac{{x^2+x-12}}{x^2-6x+9} 
$$
We always do direct substitution first:
$$
\lim_{ x \to 3 } \frac{0}{0} 
$$
This is case b! (so we need to factor)
$$
\lim_{ x \to 3 } \frac{{(x+4)(x-3)}}{(x-3)(x-3)} 
$$
2 of the x-3's cancel
$$
\lim_{ x \to 3 } \frac{x+4}{x-3} 
$$
Back to direct substitution:
$$
\lim_{ x \to 3 } \frac{7}{0} 
$$
We don't have a zero on top so we approach it from both sides:
Left:
$$
\lim_{ x \to 3^- } \frac{{(x+4)(x-3)}}{(x-3)(x-3)} = - \infty
$$
x+4 is positive
x-3 on top is negative
x-3's on bottom are positive because they equal (x-3)^2 and squared is always positive

Right:
$$
\lim_{ x \to 3^+ } \frac{{(x+4)(x-3)}}{(x-3)(x-3)} = + \infty
$$
x+4 is positive
x-3 on top is positive
x-3's on bottom are positive because they equal $(x-3)^2$ and squared is always positive

They are different so $\lim_{ x \to 3 } = DNE$

##### Example 5:
$$
\lim_{ x \to 2 } \frac{{x^2 -9}}{x-2} 
$$
With direct substitution 
$$
\lim_{ x \to 2 } -\frac{5}{0} 
$$
Before approaching from the left and right, we can actually do difference of squares on top:
$$
\lim_{ x \to 2 } \frac{{(x-3)(x+3)}}{x-2} 
$$
Left:
$$
\lim_{ x \to 2^- } \frac{{(x-3)(x+3)}}{x-2} = - \infty
$$
x-3 is negative
x+3 is positive
x-2 is negative
Right:
$$
\lim_{ x \to 2^+ } \frac{{(x-3)(x+3)}}{x-2} = + \infty
$$
x-3 is negative
x+3 is positive
x-2 is positive

They are different so $\lim_{ x \to 2 } = DNE$
## Absolute Value
---
##### Example 1:
$$
f(x) = |x| = \begin{cases}
-x \ if \ x < 0  \\
x \ if \ x \geq 0
\end{cases} 
$$
$$
\lim_{ x \to 0 } |x| = 0
$$
$$
\lim_{ n \to 0^- } |x| = \lim_{ x \to 0^- } -x = 0  
$$
$$
\lim_{ n \to 0^+ } |x| = \lim_{ x \to 0^+ } x = 0  
$$
##### Example 2:
$$
\lim_{ x \to 0 } \frac{{|x|}}{x}
$$
$$
\frac{{|x|}}{x} = \begin{cases}
-1 \ if \ x < 0  \\
1 \ if \ x > 0
\end{cases}
$$
$$
\lim_{ x \to 0^- } -1 = -1 
$$
$$
\lim_{ x \to 0^+ } 1 = 1
$$
1 doesn't equal -1 so $\lim_{ x \to 0 } \frac{{|x|}}{x} = DNE$

##### Example 3:
>[!RULE] When it's the absolute value of the whole function
>$$
|f(x)| = \begin{cases}
f(x) \ if \ f(x) \geq 0 \\
-f(x) \ if \ f(x) < 0
\end{cases}
$$

So in this example
$$
\frac{{2x+12}}{|x+6|}
$$
If $x + 6 \geq 0$:
$$
\frac{{2x+12}}{x+6}
$$
Or if $x+6 < 0$:
$$
\frac{{2x+12}}{-(x+6)}
$$
$$
\frac{{2x+12}}{|x+6|} = \begin{cases}
\frac{{2x+12}}{x+6} \ if \ x > -6 \\
\frac{{2x+12}}{-(x+6)} \ if \ x < -6
\end{cases}
$$

## Squeeze Theorem
---
If $f(x)\leq g(x)\leq h(x)$ near a,
and $\lim_{ x \to a }f(x) = \lim_{ x \to a }h(x) = L$,
then $\lim_{ x \to a }g(x)=L$

##### Example:
$$
\lim_{ x \to 0 } {x^2\sin}{\frac{1}{x}}
$$
> [!TIP] Helpful hint
> sin or cos is a good indication that this is a squeeze theorem problem

$$
-1\leq \sin{\frac{1}{x}}\leq 1
$$
$$
-x^2\leq x^2\sin{\frac{1}{x}}\leq x^2
$$
$$
\lim_{ x \to 0 }(-x^2) \leq \lim_{ x \to 0 } x^2 \sin {\frac{1}{x}} \leq \lim_{ x \to 0 } x^2  
$$
So the original limit is
$$
\lim_{ x \to 0 } x^2 \sin {\frac{1}{x}} = 0 
$$

Steps:
1. $1\leq \cos or\sin\leq 1$
2. Turn cos/sin into f
3. Take limits of the outsides
4. Compare the 2 limits
