## Tangent Lines:
---
The tangent line to $f(x)$ at $x=a$ is a line through $(a,f(a))$ with the same slope as $f$ at $a$.
##### Example 1:
Slope of our tangent line:
$$
m=\lim_{ x \to a } \frac{{f(x)-f(a)}}{x-a} 
$$
Tangent line to $x^2$ at $(1,1), a=1$

$$
m=\lim_{ x \to 1 } \frac{{x^2-1}}{x-1} 
$$
$$
= \lim_{ x \to 1 } \frac{{(x+1)(x-1)}}{x-1} 
$$
$$
=2
$$
To find the equation we use the Point Slope formula
> [!NOTE] Point Slope
> $$
> y-y_{1} = m(x-x_{1})
> $$

### Limit definition of the derivative
$$
\frac{\Delta y}{\Delta x} = \frac{{f(x+h) - f(x)}}{h}
$$
$$
f'(x) = \lim_{ h \to 0 } \frac{{f(x+h) - f(x)}}{h} 
$$
The derivative of f

##### Example 1:
$$
f(x) = x^2
$$
$$
f'(x) = \lim_{ h \to 0 } \frac{{(x+h)^2 - x^2}}{h} 
$$
$$
= \lim_{ x \to h } \frac{{x^2+2hx + h^2 - x^2}}{h} 
$$
$$
= 2x
$$
##### Example 2:
$$
f(x) = x^2 - x
$$
$$
f'(x)= \lim_{ h \to 0 } \frac{{(x+h)^2-(x+h)-(x^2-x)}}{h}
$$
$$
=\lim_{ h \to 0 } \frac{{x^2+2hx+h^2-x-h-x^2+x}}{h}
$$
$$
= \lim_{ h \to 0 } \frac{{2hx+h^2-h}}{h}
$$
$$
= \lim_{ h \to 0 } \frac{{h(2x+h-1)}}{h}
$$
$$
= 2x-1
$$
##### Example 3:
$$
g(x) = \sqrt{ x }
$$
$$
g'(x) = \lim_{ h \to 0 } \frac{{\sqrt{ x+h } - \sqrt{ x }}}{h}
$$
$$
= \lim_{ h \to 0 } \frac{{\sqrt{ x+h } - \sqrt{ x }}}{h} \frac{{(\sqrt{ x+h } + \sqrt{ x })}}{(\sqrt{ x+h } + \sqrt{ x })}
$$
$$
= \lim_{ h \to 0 } \frac{{x+h-\sqrt{ x }\sqrt{ x+h }+\sqrt{ x }\sqrt{ x+h }-x}}{h(\sqrt{ x+h }+\sqrt{ x })}
$$
$$
= \lim_{ h \to 0 } \frac{{h}}{h(\sqrt{ x+h }+\sqrt{ x })}
$$
$$
= \lim_{ h \to 0 } \frac{1}{\sqrt{ x+h }+\sqrt{ x }}
$$
$$
= \frac{1}{2}x^{-1/2}
$$
## Rate of Change
---
$y=f(x)$
$\Delta x$ is a change in $x$
$\Delta y$ is a change in $y$
$\frac{{\Delta y}}{\Delta x}$ = average rate of change of $y$ as $x$ changes from $x_{1}$ to $x_{2}$

$f'(x) = \lim_{ \Delta x \to 0 } \frac{{\Delta y}}{\Delta x}$
the instantaneous rate of change of $y$ with respect to $x$ 

##### Position:
$p(t)$ = position at time $t$
$p'(t)$ = rate of change of position = velocity = $v(t)$
$v'(t)$ = rate of change of velocity = acceleration = $a(t)$
$a'(t)$ = rate of change of acceleration = jerk = $j(t)$
