$$
F(x) = \sqrt{ x^2 + 1 }
$$
$$
F(x) = fog(x) = f(g(x))
$$
$$
F'(x) = \frac{dy}{dx}=\frac{dy}{du} \frac{dy}{dx}
$$
Steps:
1. Identify the "outside" function (the f)
2. Take the derivative of the outside leaving the inside alone (power rule)
3. Multiply the derivative of the inside

Example 1:
$$
f(x) = (x^2 + 1)^{1/2}
$$
$$
f'(x) = \frac{1}{2}(x^2+1)^{-{1/2}}(2x)
$$
Example 2:
$$
y = \sin(x^2)
$$
$$
y' = \cos(x^2)(2x)
$$
Example 3:
$$
y = \sin^2x
$$
$$
= (\sin x)^2
$$
$$
y' = 2(\sin x)(\cos x)
$$
Example 4:
$$
y = (x^2 + 2x + 10)^{100}
$$
$$
y' = 100(x^2+2x+10)^{99}(2x+2)
$$
Example 5:
$$
f(x) = \frac{1}{\sqrt[3]{ x^3 - 10x + 1 }}
$$
$$
= (x^3-10x+1)^{-1/3}
$$
$$
f'(x) = -\frac{1}{3}(x^3-10x+1)^{-\frac{4}{3}}(3x^2-10)
$$
## Implicit Differentiation
---
> [!NOTE] When to use
> Use this when x's and y's are kinda just all over the place in the problem!


$$
[f(g(x))]' = f'(g(x))g'(x)
$$
1. Take x derivatives like normal
2. The y derivatives but multiply by $\frac{dy}{dx}$
3. Solve for $\frac{dy}{dx}$
##### Example 1:
$$
x^2+y^2=16
$$
Instead of getting y by itself and taking the derivative, we can just take the derivative of everything and multiply y by $\frac{dy}{dx}$
$$
2x + (2y\frac{dy}{dx}) = 0
$$
Then get $\frac{dy}{dx}$ by its self
$$
\frac{dy}{dx} = -\frac{x}{y}
$$
##### Example 2 (Folium of Descartes):
$$
x^3 + y^3 = 6xy
$$
$$
3x^2 + (3y^2 {\frac{dy}{dx}}) = 6y+6x (\frac{dy}{dx})
$$
$$
3y^2 (\frac{dy}{dx}) - 6x (\frac{dy}{dx}) = 6y - 3x^2
$$
$$
\left( \frac{dy}{dx} \right)(3y^2 - 6x) = 6y - 3x^2
$$
$$
\frac{dy}{dx} = \frac{{6y-3x^2}}{3y^2-6x}
$$
##### Example 3 (find y''):
$$
x^4 + y^4 = 16
$$
$$
4x^3 + 4y^3 \left( \frac{dy}{dx} \right) = 0
$$
$$
4y^3 \left( \frac{dy}{dx} \right) = -4x^3
$$
$$
\frac{dy}{dx} = -\frac{x^3}{y^3}
$$
$$
\frac{d^2y}{d^2x} = -\frac{{(y^3)(3x^2)-(x^3)(3y^2(\frac{dy}{dx}))}}{y^6}
$$
Substitute $\frac{dy}{dx}$ with what we got in a previous step
$$
\frac{{d^2y}}{d^2x} = - \frac{{3x^2y^3 - 3y^2x^3\left( -\frac{x^3}{y^2} \right)}}{y^6}
$$

