##### Example 1:
Find asymptotes for
$$
\frac{{\sqrt{ 7+9x^2 }}}{1-2x}
$$

Vertical asymptotes can be determined by getting whatever x is that makes the denominator equal to 0.

V.A $x=\frac{1}{2}$


$$
\lim_{ x \to \infty } \frac{{\sqrt{ 7+9x^2 }}}{1-2x}
$$
Multiply by 1/x because x is the highest power

$$
\lim_{ x \to \infty } \frac{{\sqrt{ 7+9x^2 }}}{1-2x} \frac{{\frac{1}{x}}}{\frac{1}{x}}
$$
$$
\lim_{ x \to \infty } \frac{{\sqrt{ \frac{7}{x^2} + 9}}}{\frac{1}{x} - 2}
$$
$$
= \frac{{\sqrt{ 0+9 }}}{0-2} = -\frac{3}{2}
$$
H.A. $y = - \frac{3}{2}$
But we also need to take the limit to negative infinity

$$
\lim_{ x \to -\infty } \frac{{\sqrt{ 7+9x^2 }}}{1-2x}
$$
Process is the same
$$
\lim_{ x \to \infty } \frac{{\sqrt{ \frac{7}{x^2} + 9}}}{\frac{1}{x} - 2}
$$
Since its the limit to negative infinity we can look at the original denominator and see if the sign changes when we plug in a negative number. In this case $1-2(neg)$ will be a positive so the sign changes, so we have to make the denominator negative in our answer.
$$
= \frac{{\sqrt{ 0+9 }}}{-(0-2)} = \frac{3}{2}
$$
