![[Pasted image 20231127120728.png]]
$$
A = \int_{a}^b f(x)  \, dx - \int_{a}^b g(x) \, dx 
$$
$$
 = \int _{a}^b (f(x)- g(x)) \, dx 
$$
If the second curve (g(x)) is negative (under the x axis) then it will be added to the top curve (f(x))

##### Example 1
$y = x^2 + 1$
$y = x$
$x = 0, x=1$

$x^2 + 1$ is on top, $y=x$ is on bottom. I need to find the area in between the points 0 and 1.

$$
A = (x^2 + 1 - x)\Delta x
$$
Turn into integral and solve:
$$
\int _{0}^1 x^2 + 1 -x \, dx 
$$
$$
=\frac{x^3}{3} + x - \frac{x^2}{2}
$$
$$
=\frac{1}{3}+1- \frac{1}{2} - 0
$$
$$
= \frac{5}{6}
$$

##### Example 2
$y = x^2$
$y=2x-x^2$
If you aren't given the left and right endpoints, you typically have to solve for them.

Endpoints (find where they meet):
$$
2x-x^2 = x^2
$$
$$
2x-2x^2 = 0
$$
$$
2x(1-x) = 0
$$
$$
x = 0, x = 1
$$
Solve:
$$
A = (2x-x^2 - x^2)\Delta x
$$
$$
\int _{0}^1 (2x-x^2 - x^2) \, dx 
$$
$$
= x^2 - \frac{2x^3}{3}
$$
$$
(1)^2 - \frac{2(1)^3}{3} - (0)^2 - \frac{2(0)^3}{3}
$$
$$
= \frac{1}{3}
$$

##### Example 3
$y = \sin x$
$y = \cos x$
$x = 0$
$x = \frac{\pi}{2}$


The top and bottom curve change so we need to take 2 integrals and add them

First we need to find the point where they're equal

$\sin x = \cos x$
$x = \frac{\pi}{4}$

$$A = (\cos x - \sin x)\Delta x$$
$$
\int _{0}^{\pi/4} (\cos x -\sin x) \, dx 
$$
$$
\int _{\frac{\pi}{4}}^{\pi/2} (\sin x - \cos x) \, dx 
$$

Final setup:
$$
\int _{0}^{\pi/4} (\cos x -\sin x) \, dx + \int _{\frac{\pi}{4}}^{\pi/2} (\sin x - \cos x) \, dx 
$$

##### Example 4
$y = \sin x$
$y = \cos x$
$y = 0$
$x=0,x=\frac{\pi}{2}$

![[Pasted image 20231127125559.png]]
$$
A = \int _{0}^{\pi/4} \sin x \, d + \int _{\frac{\pi}{4}}^{\pi/2}\cos x \, dx  
$$
##### Example 5
$y=x-1$
$y^2 = 2x+6$ (Since there's gonna be 2 answers, a pos sqrt and a neg sqrt. Its just gonna be a sideways parabola)

$$
x = y + 1
$$
$$
y + 1 = \frac{y^2}{2} - 3
$$
$$
y = -2, y = 4
$$

We're going to write the area in terms of y, since its sideways

$$
A = y+1 -\left( \frac{y^3}{3} -3 \right) \Delta y
$$
$$
\int _{-2}^4 (y+1 -\left( \frac{y^3}{3} -3 \right)) \, dy
$$
