
## Distributive Law
****
$$ a(b+c) = ab + ac $$
#### Ex 1.
$$ (x+2)(3x-5) = 3x^2 - 5x + 6x - 10 $$
#### Ex 2.
$$ (x-3)^2 = (x-3)(x-3) $$


> [!NOTE] How to simplify this easier
> You can use the idea of $$ (a+b)^2 = a^2 + 2ab + b^2 $$
> to simplify this easier

## Fractions
****
#### Adding fractions

When the denominators are alike:
$$ \frac{a}{b} + \frac{c}{b} = \frac{a+c}{b} $$
When the denominators are different:

#### Ex 1.
Find common denominators
$$ \frac{1}{2} + \frac{1}{3} $$
Make them the same denominators
$$ \frac{1*3}{2*3} + \frac{1*3}{3*3} = \frac{3}{6} + \frac{2}{6} = \frac{5}{6} $$
#### Ex 2.
Need to make this one fraction using the same idea
$$ \frac{3}{(x-1)} + \frac{x}{(x+2)} $$
$$ = \frac{3(x+2) + x(x-1)} {(x+2)(x-1)} $$
$$ = \frac{x^2 + 2x +6} {(x+2)(x-1)} $$

> [!NOTE] Rule when canceling tops and bottoms
> When you're adding terms on both the top and bottom you cant cancel stuff
> You can only cancel when they're multiplied

Multiplying factions by each other
$$ \frac{a}{b} * \frac{c}{d} $$
$$ = \frac{ac}{bd} $$
Diving Fractions by another fraction
$$ \frac{\frac{a}{b}}{\frac{c}{d}} $$
Stay change flip


## Factoring
****
#### Ex 1.
$$ 3x^2-6x $$
1. Take out GCF (Greatest Common Factor)
$$ = 3x (x-2) $$
#### Ex 2.
$$ 2x^2 + x $$
1. Take out GCF
$$ = x (2x+1) $$

> [!NOTE] Note
> When taking out an x from just a single x remember that there still is a 1 there.


#### Ex 3.
$$ x^2 + bx + c $$
Adds to b
Multiplies to c

$$ x^2 +5x -24 $$
$$ = (x + 8)(x - 3) $$
These 2 numbers should add to the middle number
These 2 numbers should multiply to the last number
$$ 8 * -3 = -24 $$
$$ 8 + -3 = 5 $$
> [!NOTE] This only applies if there is no number in front of the first term!

#### Ex 4.
$$ 2x^2 - 7x -4 $$
This can be solved by using the ac method!

Multiply to ac
Add to b
$$ 1 * -8 = -8 $$
$$ 1 + -8 = -7 $$
Factoring by grouping
$$ 2x + 1x - 8x - 4 $$
$$ x(2x+1) -4(2x+1) $$
$$ = (2x +1)(x-4) $$
> [!NOTE] These 2 terms have to be the same to work!

#### Difference of squares
$$ a^2 - b^2 $$
$$ = (a+b)(a-b) $$
#### Difference of cubes
$$ a^3 + b^3 $$
$$ = (a + b)(a^2-2ab+b^2) $$
$$ a^3 - b^3 $$
$$ = (a - b)(a^2+2ab+b^2) $$
> [!NOTE] Way to remember signs for difference of cubes
> Same, opposite, always positive

#### Ex 5.
$$ \frac{x^2 - 16}{x^2 - 2x - 8} $$
Factor both terms
$$ x^2 - 16 $$
$$ = (x+4)(x-4) $$
$$ (x^2 -2x -8) $$
$$ = (x-4)(x+2)$$
Adds to -2
Multiplies to -8

$$ \frac{(x+4)(x-4)}{(x-4)(x+2)} $$
Same cancels since its multiplying
$$ = \frac{(x+4)}{(x+2)} $$